module STLC where

open import Data.Bool using (_∨_; _∧_; if_then_else_)
open import Data.List using (List; []; [_]; _++_; filter)
open import Data.String using (String; _≟_; _==_)
open import Data.Product using (_×_; _,_; proj₁; proj₂)
open import Relation.Nullary using (¬?; ⌊_⌋)
open import Relation.Binary.PropositionalEquality using (_≡_; refl; cong; cong₂)

open import Data.List.Membership.DecPropositional _≟_ using (_∈?_; _∉?_)

-- 1.1.1: The set of untyped λ-terms
V : Set
V = String

data Λ : Set where
  `_   : V → Λ
  ƛ_⇒_ : V → Λ → Λ
  _·_  : Λ → Λ → Λ

-- 1.1.2: Notation
infix  9 `_
infixl 7 _·_
infixr 5 ƛ_⇒_

private
  variable
    L M N P Q R : Λ
    x y z u v w : V

-- 1.1.3:
-- i: Free variables
FV : Λ → List V
FV (` x)     = [ x ]
FV (ƛ x ⇒ P) = filter (λ y → ¬? (x ≟ y)) (FV P)
FV (P · Q)   = FV P ++ FV Q

-- ii: Closed; Combinator
Closed : Λ → Set
Closed M = FV M ≡ []

-- 1.1.4: Equality
-- congruence
`-cong : x ≡ y → ` x ≡ ` y
`-cong = cong `_

ƛ-cong : x ≡ y → M ≡ N → ƛ x ⇒ M ≡ ƛ y ⇒ N
ƛ-cong = cong₂ ƛ_⇒_

ƛ-cong-binder : x ≡ y → ƛ x ⇒ M ≡ ƛ y ⇒ M
ƛ-cong-binder h = ƛ-cong h refl

ƛ-cong-body : M ≡ N → ƛ x ⇒ M ≡ ƛ x ⇒ N
ƛ-cong-body = ƛ-cong refl

·-cong : M ≡ N → P ≡ Q → M · P ≡  N · Q
·-cong = cong₂ _·_

·-cong-left : M ≡ N → M · L ≡ N · L
·-cong-left h = ·-cong h refl

·-cong-right : M ≡ N → L · M ≡ L · N
·-cong-right = ·-cong refl

-- injectivity
`-inj : ` x ≡ ` y → x ≡ y
`-inj refl = refl

ƛ-inj : ƛ x ⇒ M ≡ ƛ y ⇒ N → x ≡ y × M ≡ N
ƛ-inj refl = refl , refl

ƛ-inj-binder : ƛ x ⇒ M ≡ ƛ y ⇒ N → x ≡ y
ƛ-inj-binder h = proj₁ (ƛ-inj h)

ƛ-inj-body : ƛ x ⇒ M ≡ ƛ y ⇒ N → M ≡ N
ƛ-inj-body h = proj₂ (ƛ-inj h)

·-inj : M · P ≡ N · Q → M ≡ N × P ≡ Q
·-inj refl = refl , refl

·-inj-left : M · L ≡ N · L → M ≡ N
·-inj-left h = proj₁ (·-inj h)

·-inj-right : L · M ≡ L · N → M ≡ N
·-inj-right h = proj₂ (·-inj h)

-- 1.1.5: β-reduction and η-reduction
-- substitution
_[_:=_] : Λ → V → Λ → Λ
(` y)     [ x := N ] = if x == y then N else ` y
(ƛ y ⇒ M) [ x := N ] = if (x == y) ∨ ⌊ y ∈? FV N ⌋ then ƛ y ⇒ M else ƛ y ⇒ M [ x := N ]
(M · L)   [ x := N ] = M [ x := N ] · L [ x := N ]

infix 9 _[_:=_]

-- β-rule
β⟶_ : Λ → Λ
β⟶ ((ƛ x ⇒ M) · N) = M [ x :=  N ]
β⟶ (` x)           = ` x
β⟶ (ƛ x ⇒ M)       = ƛ x ⇒ β⟶ M
β⟶ (M · N)         = β⟶ M · β⟶ N

-- η-rule
η⟶_ : Λ → Λ
η⟶ (ƛ x ⇒ M · ` y) = if (x == y) ∧ ⌊ x ∉? FV M ⌋ then M else ƛ x ⇒ M · ` y
η⟶ (` x)           = ` x
η⟶ (ƛ x ⇒ M)       = ƛ x ⇒ η⟶ M
η⟶ (M · N)         = η⟶ M · η⟶ N

module Combinators where
  I = ƛ "x" ⇒ ` "x"
  K = ƛ "x" ⇒ ƛ "y" ⇒ ` "x"
  S = ƛ "x" ⇒ ƛ "y" ⇒ ƛ "z" ⇒ ` "x" · ` "z" · (` "y" · ` "z")

  Ω = (ƛ "x" ⇒ ` "x" · ` "x") · (ƛ "x" ⇒ ` "x" · ` "x")
  Y = ƛ "f" ⇒ (ƛ "x" ⇒ ` "f" · (` "x" · ` "x")) · (ƛ "x" ⇒ ` "f" · (` "x" · ` "x"))
